most of completeness

Clean/Gadgets/Xor/ByteXorTable.lean
@@ -10,13 +10,43 @@ variable [p_large_enough: Fact (p > 512)]
 def from_byte (x: Fin 256) : F p :=
   FieldUtils.nat_to_field x.val (by linarith [x.is_lt, p_large_enough.elim])
 
+lemma from_byte_eq (x : F p) (x_lt : x.val < 256) : from_byte ⟨ x.val, x_lt ⟩ = x := by
+  dsimp [from_byte]
+  sorry
+
+omit [Fact (p ≠ 0)] in
+lemma from_byte_cast_eq {z: F p} (z_lt : z.val < 256) : from_byte z.cast = z := by
+  simp only [from_byte]
+  have : (z.cast : Fin 256).val = z.val := ZMod.val_cast_eq_val_of_lt z_lt
+  simp only [this]
+  apply FieldUtils.nat_to_field_of_val_eq_iff
+
+def split_two_bytes (i : Fin (256 * 256)) : (Fin 256 × Fin 256) :=
+  let x := i.val / 256
+  let y := i.val % 256
+  have x_lt : x < 256 := by simp [x, Nat.div_lt_iff_lt_mul]
+  have y_lt : y < 256 := Nat.mod_lt i.val (by norm_num)
+  (⟨ x, x_lt ⟩, ⟨ y, y_lt ⟩)
+
+def concat_two_bytes (x y : Fin 256) : Fin (256 * 256) :=
+  let i := x.val * 256 + y.val
+  have i_lt : i < 256 * 256 := by sorry
+  ⟨ i, i_lt ⟩
+
+lemma concat_split_1 (x y : Fin 256) : (split_two_bytes (concat_two_bytes x y)).1 = x := by
+  dsimp [split_two_bytes, concat_two_bytes]
+  sorry
+
+lemma concat_split_2 (x y : Fin 256) : (split_two_bytes (concat_two_bytes x y)).2 = y := by
+  dsimp [split_two_bytes, concat_two_bytes]
+  sorry
+
 def ByteXorTable: Table (F p) where
   name := "ByteXor"
   length := 256*256
   arity := 3
   row i :=
-    let x := i / 256
-    let y := i % 256
+    let (x, y) := split_two_bytes i
     #v[from_byte x, from_byte y, from_byte (Nat.xor x y)]
 
 def ByteXorTable.soundness
@@ -36,25 +66,15 @@ def ByteXorTable.completeness
     z.val = Nat.xor x.val y.val → ByteXorTable.contains (#v[x, y, z]) := by
   intro h
   dsimp only [ByteXorTable, Table.contains]
-  use x.val * 256 + y.val
-  simp [from_byte, Vector.eq_mk, Array.mk.injEq, List.cons.injEq, and_true, Fin.val_cast_of_lt hx]
+  use concat_two_bytes ⟨ x.val, hx ⟩ ⟨ y.val, hy ⟩
+  simp only [Vector.eq_mk, Array.mk.injEq, List.cons.injEq, and_true]
+  rw [concat_split_1, concat_split_2]
+  simp only [from_byte_eq, true_and]
 
-  have h_x' : x.val % 256 = x.val := by
-    apply (Nat.mod_eq_iff_lt (by linarith)).mpr
-    exact hx
-
-  -- have h_xy : (Fin.val ((ZMod.cast x : Fin 65536) * 256 + ZMod.cast y) / ↑256) % 256 = ZMod.cast x := by
-    -- sorry
-
-  have sanity : ((ZMod.cast x) * 256 : Fin 65536) + ZMod.cast y = 0 := by sorry
-
-
-  have h_y' : y.val % 256 = y.val := by
-    apply (Nat.mod_eq_iff_lt (by linarith)).mpr
-    exact hy
-
-  constructor
-  rw [sanity]
+  have hz : z.val < 256 := by sorry
+  rw [←h]
+  simp only [ZMod.natCast_val]
+  rw [from_byte_cast_eq hz]
 
 def ByteXorTable.equiv (x y z: F p) (hx : x.val < 256) (hy : y.val < 256) :
     ByteXorTable.contains (#v[x, y, z]) ↔ z.val = Nat.xor x.val y.val :=
